pprog + review comments applied

txn-data-consistency/ProgrammingLanguage.thy
@@ -44,10 +44,22 @@ definition kvs_init :: "'v kv_store" where
 
 \<comment> \<open>predicates on kv stores\<close>
 
-(*
-  Formalize the conditions (snapshot), (rw-so), (ww-so) from p9 of ECOOP paper;
-  see also Def 4.5 of Xiong's PhD thesis, which defines well-formedness of kv stores.
-*)
+definition snapshot_property :: "'v kv_store \<Rightarrow> bool" where
+  "snapshot_property K \<equiv>
+    \<forall>k i j. v_readerset (K k!i) \<inter> v_readerset (K k!j) \<noteq> {} \<or>
+            v_writer (K k!i) = v_writer (K k!i) \<longrightarrow> i = j"
+
+definition SO :: "txid0 rel" where
+  "SO \<equiv> {(t, t'). \<exists>cl n m. t = Tn_cl n cl \<and> t' = Tn_cl m cl \<and> n < m}"
+
+definition wr_so :: "'v kv_store \<Rightarrow> bool" where
+  "wr_so K \<equiv> \<forall>k i t t'. Tn t = v_writer (K k!i) \<and> t' \<in> v_readerset (K k!i) \<longrightarrow> (t', t) \<notin> SO^="
+
+definition ww_so :: "'v kv_store \<Rightarrow> bool" where
+  "ww_so K \<equiv> \<forall>k i j t t'. Tn t = v_writer (K k!i) \<and> Tn t' = v_writer (K k!j) \<and> i < j \<longrightarrow> (t', t) \<notin> SO^="
+
+definition wellformed :: "'v kv_store \<Rightarrow> bool" where \<comment>\<open>Where should this be checked?\<close>
+ "wellformed K \<equiv> snapshot_property K \<and> wr_so K \<and> ww_so K \<and> (\<forall>k. K (k!0) = undefined)"
 
 
 \<comment> \<open>functions on kv stores\<close>
@@ -64,17 +76,6 @@ definition kvs_txids :: "'v kv_store \<Rightarrow> txid set" where
 definition get_sqns :: "'v kv_store \<Rightarrow> cl_id \<Rightarrow> sqn set" where
   "get_sqns kvs cl \<equiv> {n. Tn (Tn_cl n cl) \<in> kvs_txids kvs}"
 
-(* replace the following teo defs by the one below (fresh_txids) *)
-definition next_sqn :: "'v kv_store \<Rightarrow> cl_id \<Rightarrow> sqn" where
-  "next_sqn kvs cl \<equiv> (if get_sqns kvs cl = {} then 0 else Max (get_sqns kvs cl) + 1)"
-
-abbreviation next_txid :: "'v kv_store \<Rightarrow> cl_id \<Rightarrow> txid0" where
-  "next_txid kvs cl \<equiv> Tn_cl (next_sqn kvs cl) cl"
-
-(*
-  alternatively, fresh txids could be obtained from the following set, i.e., 
-  as t \<in> next_txids kvs cl, which reflect the paper's more abstract definition
-*)
 definition next_txids :: "'v kv_store \<Rightarrow> cl_id \<Rightarrow> txid0 set" where
   "next_txids kvs cl \<equiv> {Tn_cl n cl | n cl. \<forall>m \<in> get_sqns kvs cl. m < n}"
 
@@ -83,47 +84,30 @@ subsection \<open>Views\<close>
 
 type_synonym v_id = nat
 
-type_synonym views = "key \<Rightarrow> v_id set"
+type_synonym view = "key \<Rightarrow> v_id set"
 
-definition views_init :: views where
-  "views_init _ \<equiv> {0}"
+definition view_init :: view where
+  "view_init _ \<equiv> {0}"
 
-definition view_order :: "views \<Rightarrow> views \<Rightarrow> bool" (infix "\<sqsubseteq>" 60) where
+definition view_order :: "view \<Rightarrow> view \<Rightarrow> bool" (infix "\<sqsubseteq>" 60) where
   "u1 \<sqsubseteq> u2 \<equiv> \<forall>k. u1 k \<subseteq> u2 k"
 
-(*
-  define here:
-  - the predicates view_in_range and view_atomic 
-  from Definition 2 (ECOOP) 
-*)
+definition view_in_range :: "'v kv_store \<Rightarrow> view \<Rightarrow> bool" where \<comment>\<open>Where should this be checked?\<close>
+  "view_in_range K u \<equiv> \<forall>k i. 0 \<in> u k \<and>  (i \<in> u k \<longrightarrow> 0 \<le> i \<and> i < length (K k))"
+
+definition view_atomic :: "'v kv_store \<Rightarrow> view \<Rightarrow> bool" where \<comment>\<open>Where should this be checked?\<close>
+  "view_atomic K u \<equiv> \<forall>k k' i i'. i \<in> u k \<and> v_writer (K k!i) = v_writer (K k'!i') \<longrightarrow> i' \<in> u k'"
 
 
 subsection \<open>Operational semantics\<close>
 
-(* config type is never used in operational semantics rules below *)
-
-record 'v config =
-  c_kvs :: "'v kv_store"
-  c_conf :: "cl_id \<Rightarrow> views"
-
-definition conf_init :: "cl_id \<Rightarrow> views" where
-  "conf_init _ \<equiv> views_init"
-
-definition config_init :: "'v config" where
-  "config_init \<equiv> \<lparr>c_kvs = kvs_init, c_conf = conf_init\<rparr>"
-
-
 type_synonym 'v snapshot = "key \<Rightarrow> 'v"
 
-definition last_version :: "'v kv_store \<Rightarrow> views \<Rightarrow> key \<Rightarrow> 'v version" where
+definition last_version :: "'v kv_store \<Rightarrow> view \<Rightarrow> key \<Rightarrow> 'v version" where
   "last_version kvs u k \<equiv> kvs k!(Max (u k))"
 
-definition view_snapshot :: "'v kv_store \<Rightarrow> views \<Rightarrow> 'v snapshot" where
+definition view_snapshot :: "'v kv_store \<Rightarrow> view \<Rightarrow> 'v snapshot" where
   "view_snapshot kvs u k \<equiv> v_value (last_version kvs u k)"
-
-definition txn_snapshot :: "'v config \<Rightarrow> cl_id \<Rightarrow> 'v snapshot" where
-  "txn_snapshot cfg cl k \<equiv> v_value (last_version (c_kvs cfg) (c_conf cfg cl) k)"
-
 
 datatype op_type = R | W
 datatype 'v op = Read key 'v | Write key 'v | Eps
@@ -137,30 +121,12 @@ fun update_fp :: "'v fingerpr \<Rightarrow> 'v op \<Rightarrow> 'v fingerpr" whe
   "update_fp fp (Write k v) = fp ((k, W) \<mapsto> v)" |
   "update_fp fp Eps         = fp"
 
-(*
-  CHSP: I have 
-  - split the def of update_kv into two parts, one for reads and one for writes, and 
-  - reordered the arguments, in particular moved the kv_store to the last position 
-    to enable the use of function composition.
-
-  TODO: Check out whether there is a better way to update kv stores with fingerprints
-  which does not raise the well-formedness questions arising from def below.
-
-  Maybe we could drop the values read from the fingerprints (or ignore them), as they 
-  are not needed to update the kv store (maybe anywhere else?).
-
-  The way that update_kv is used the else branch below should not be needed: 
-  The kvs-view pair (K, u) to compute the snapshot on which the fingerprint is based 
-  is the same as the pair used to update the kv store using update_kv.
-*)
-fun update_kv_reads :: "txid0 \<Rightarrow> 'v fingerpr \<Rightarrow> views \<Rightarrow> 'v kv_store \<Rightarrow> 'v kv_store" where
+fun update_kv_reads :: "txid0 \<Rightarrow> 'v fingerpr \<Rightarrow> view \<Rightarrow> 'v kv_store \<Rightarrow> 'v kv_store" where
   "update_kv_reads t fp u kvs k =
     (case fp (k, R) of
       None   \<Rightarrow> kvs k |
       Some v \<Rightarrow> let lv = last_version kvs u k in
-                  if v = v_value lv
-                  then (kvs k)[Max (u k) := lv\<lparr>v_readerset := insert t (v_readerset lv)\<rparr>]
-                  else kvs k)"   \<comment>\<open>Throwing an exception? t has read the wrong value\<close>
+                  (kvs k)[Max (u k) := lv\<lparr>v_readerset := insert t (v_readerset lv)\<rparr>])"
 
 fun update_kv_writes :: "txid0 \<Rightarrow> 'v fingerpr \<Rightarrow> 'v kv_store \<Rightarrow> 'v kv_store" where
   "update_kv_writes t fp kvs k =
@@ -168,7 +134,7 @@ fun update_kv_writes :: "txid0 \<Rightarrow> 'v fingerpr \<Rightarrow> 'v kv_sto
       None   \<Rightarrow> kvs k |
       Some v \<Rightarrow> kvs k @ [\<lparr>v_value=v, v_writer=Tn t, v_readerset={}\<rparr>])"
 
-definition update_kv :: "txid0 \<Rightarrow> 'v fingerpr \<Rightarrow> views \<Rightarrow> 'v kv_store \<Rightarrow> 'v kv_store" where
+definition update_kv :: "txid0 \<Rightarrow> 'v fingerpr \<Rightarrow> view \<Rightarrow> 'v kv_store \<Rightarrow> 'v kv_store" where
   "update_kv t fp u = (update_kv_writes t fp) o (update_kv_reads t fp u)"
 
 
@@ -180,20 +146,15 @@ inductive cp_step :: "'a \<Rightarrow> 'a cmd_p \<Rightarrow> 'a \<Rightarrow> b
 
 \<comment> \<open>primitives transactions\<close>
 
-(* could define semantics of Assign and Assume steps in terms of cp_step to avoid redundancy *)
 inductive tp_step :: "'a \<Rightarrow> 'v snapshot \<Rightarrow> ('a, 'v) txn_p \<Rightarrow> 'a \<Rightarrow> 'v snapshot \<Rightarrow> bool" where
-  "tp_step s \<sigma> (TCp (Assign f)) (f s) \<sigma>" |
-  "t s \<Longrightarrow> tp_step s \<sigma> (TCp (Assume t)) s \<sigma>" |
   "tp_step s \<sigma> (Lookup k f_rd) (f_rd (\<sigma> k) s) \<sigma>" |
-  "\<sigma>' = \<sigma>(k := f_wr s) \<Longrightarrow> tp_step s \<sigma> (Mutate k f_wr) s \<sigma>'"
+  "\<sigma>' = \<sigma>(k := f_wr s) \<Longrightarrow> tp_step s \<sigma> (Mutate k f_wr) s \<sigma>'"|
+  "cp_step s cp s' \<Longrightarrow> tp_step s \<sigma> (TCp cp) s' \<sigma>"
 
-(* could use wild card for first two cases (see below) *)
 fun get_op :: "'a \<Rightarrow> 'v snapshot \<Rightarrow> ('a, 'v) txn_p \<Rightarrow> 'v op" where
-  "get_op s \<sigma> (TCp (Assign f)) = Eps" |
-  "get_op s \<sigma> (TCp (Assume t)) = Eps" |
   "get_op s \<sigma> (Lookup k f_rd)  = Read k (\<sigma> k)" |
-  "get_op s \<sigma> (Mutate k f_wr)  = Write k (f_wr s)"
-(*  "get_op s \<sigma> _ = Eps" *)
+  "get_op s \<sigma> (Mutate k f_wr)  = Write k (f_wr s)"|
+  "get_op s \<sigma> _ = Eps"
 
 type_synonym ('a, 'v) t_state = "('a \<times> 'v snapshot \<times> 'v fingerpr) \<times> ('a, 'v) txn"
 
@@ -213,22 +174,22 @@ fun t_multi_step :: "('a, 'v) t_state \<Rightarrow> ('a, 'v) t_state \<Rightarro
 
 subsection \<open>Execution tests and \<close>
 
-definition visTx :: "'v kv_store \<Rightarrow> views \<Rightarrow> txid set" where
+definition visTx :: "'v kv_store \<Rightarrow> view \<Rightarrow> txid set" where
   "visTx K u \<equiv> {v_writer (K k!i) | i k. i \<in> u k}"
 
 definition read_only_Ts :: "'v kv_store \<Rightarrow> txid set" where
   "read_only_Ts kvs \<equiv> kvs_txids kvs - kvs_writers kvs"
 
-definition closed :: "'v kv_store \<Rightarrow> views \<Rightarrow> txid rel \<Rightarrow> bool" where
+definition closed :: "'v kv_store \<Rightarrow> view \<Rightarrow> txid rel \<Rightarrow> bool" where
   "closed K u r \<longleftrightarrow> visTx K u = (((r^*)^-1) `` (visTx K u)) - (read_only_Ts K)" 
 
 locale ExecutionTest =
   fixes R_ET :: "'v kv_store \<Rightarrow> 'v fingerpr \<Rightarrow> txid rel"
-    and vShift :: "'v kv_store \<Rightarrow> views \<Rightarrow> 'v kv_store \<Rightarrow> views \<Rightarrow> bool"
+    and vShift :: "'v kv_store \<Rightarrow> view \<Rightarrow> 'v kv_store \<Rightarrow> view \<Rightarrow> bool"
    \<comment>\<open>We need some assumptions from Definition 8 of ECOOP paper\<close>
 begin
 
-definition canCommit :: "'v kv_store \<Rightarrow> views \<Rightarrow> 'v fingerpr \<Rightarrow> bool" where
+definition canCommit :: "'v kv_store \<Rightarrow> view \<Rightarrow> 'v fingerpr \<Rightarrow> bool" where
   "canCommit K u F \<equiv> closed K u (R_ET K F)"
 
 end
@@ -236,9 +197,28 @@ end
 interpretation ET_CC: ExecutionTest "(\<lambda>k f. {})" "(\<lambda>k u k' u'. True)" .
 
                                       
-datatype 'v label = NA cl_id | CF cl_id views "'v fingerpr"
+datatype 'v label = NA cl_id | CF cl_id view "'v fingerpr"
 
-type_synonym ('a, 'v) c_state = "('v kv_store \<times> views \<times> 'a) \<times> ('a, 'v) cmd"
+type_synonym ('a, 'v) c_state = "('v kv_store \<times> view \<times> 'a) \<times> ('a, 'v) cmd"
+
+record 'v config =
+  c_kvs :: "'v kv_store"
+  c_views :: "cl_id \<Rightarrow> view"
+
+definition c_views_init :: "cl_id \<Rightarrow> view" where
+  "c_views_init _ \<equiv> view_init"
+
+definition config_init :: "'v config" where
+  "config_init \<equiv> \<lparr>c_kvs = kvs_init, c_views = c_views_init\<rparr>"
+
+definition txn_snapshot :: "'v config \<Rightarrow> cl_id \<Rightarrow> 'v snapshot" where \<comment>\<open>Is this needed?\<close>
+  "txn_snapshot cfg cl k \<equiv> v_value (last_version (c_kvs cfg) (c_views cfg cl) k)"
+
+type_synonym 'a c_env = "cl_id \<rightharpoonup> 'a"
+
+type_synonym ('a, 'v) progs = "cl_id \<rightharpoonup> ('a, 'v) cmd"
+
+type_synonym ('a, 'v) p_state = "('v config \<times> 'a c_env) \<times> ('a, 'v) progs"
 
 
 context ExecutionTest
@@ -250,7 +230,7 @@ inductive c_step :: "('a, 'v) c_state \<Rightarrow> 'v label \<Rightarrow> ('a, 
   "cp_step s cp s' \<Longrightarrow> c_step ((K, u, s), (Cp cp)) (NA cl) ((K, u, s'), Skip)"|
   "\<lbrakk> u \<sqsubseteq> u''; \<sigma> = view_snapshot K u''; 
      t_multi_step ((s, \<sigma>, \<lambda>k. None), T) ((s', _, F), TSkip);
-     t \<in> next_txids K cl;   \<comment> \<open>was: t = next_txid K cl\<close>   
+     t \<in> next_txids K cl;
      K' = update_kv t F u'' K;
      canCommit K u F; vShift K u'' K' u' \<rbrakk>
     \<Longrightarrow> c_step ((K, u, s), Atomic T) (CF cl u'' F) ((K', u', s'), Skip)" |
@@ -264,7 +244,9 @@ inductive c_step :: "('a, 'v) c_state \<Rightarrow> 'v label \<Rightarrow> ('a, 
 
 \<comment> \<open>program semantics\<close>
 
-(* formalize rule PProg here; should use config type *)
+inductive p_prog :: "('a, 'v) p_state \<Rightarrow> ('a, 'v) p_state \<Rightarrow> bool" where
+  "u = U cl \<and> s = E cl \<and> C = P cl \<and> cp_step ((K, u, s), C) _  ((K', u', s'), C') \<and> dom P \<subseteq> dom E
+    \<Longrightarrow> p_prog ((\<lparr>c_kvs=K, c_views=U\<rparr>, E), P) ((\<lparr>c_kvs=K', c_views=U(cl := u')\<rparr>, E(cl := s')), P(cl := C'))"
 
 end
 
